

Half range Fourier Series :- If only cosine term or only sine term present in the Fourier series, then it is called Half range Fourier series :

Half range cosine series:-  $f(x) = \frac{a_0}{2} + \sum_{n=1}^{\infty} a_n \cos nx$

$$\text{where } a_0 = \frac{2}{\pi} \int_0^{\pi} f(x) dx ; a_n = \frac{2}{\pi} \int_0^{\pi} f(x) \cos nx dx$$

Half range sine series:  $f(x) = \sum_{n=1}^{\infty} b_n \sin nx$

$$\text{where } b_n = \frac{2}{\pi} \int_0^{\pi} f(x) \sin nx dx.$$

Since the function is generally defined on  $(0, \pi)$  which is half of  $(-\pi, \pi)$ . For this reason, it is called half range Fourier series.

Fourier series in Different Intervals:

(i)  $f(x)$  is defined in  $(0, \pi)$  with period  $\pi$ :

$$f(x) = \frac{a_0}{2} + \sum_{n=1}^{\infty} (a_n \cos nx + b_n \sin nx)$$

$$\text{where } a_0 = \frac{2}{\pi} \int_0^{\pi} f(x) dx ;$$

$$a_n = \frac{2}{\pi} \int_0^{\pi} f(x) \cos nx dx$$

$$b_n = \frac{2}{\pi} \int_0^{\pi} f(x) \sin nx dx.$$

(ii)  $f(x)$  is defined on  $(0, 2\pi)$  with period  $2\pi$ .

$$f(x) = \frac{a_0}{2} + \sum_{n=1}^{\infty} (a_n \cos nx + b_n \sin nx).$$

where  $a_0 = \frac{1}{\pi} \int_0^{2\pi} f(x) dx$ ;  $a_n = \frac{1}{\pi} \int_0^{2\pi} f(x) \cos nx dx$

$$b_n = \frac{1}{\pi} \int_0^{2\pi} f(x) \sin nx dx.$$

(iii)  $f(x)$  in  $(-1, 1)$  with period  $2l$ .

$\therefore f(x) = \frac{a_0}{2} + \sum_{n=1}^{\infty} (a_n \cos \frac{n\pi x}{l} + b_n \sin \frac{n\pi x}{l})$ , where  $a_0 = \frac{1}{l} \int_{-l}^l f(x) dx$

Parseval's Identity for Fourier Series  $\left\{ \begin{array}{l} a_n = \frac{1}{l} \int_{-l}^l f(x) \cos \frac{n\pi x}{l} dx \\ b_n = \frac{1}{l} \int_{-l}^l f(x) \sin \frac{n\pi x}{l} dx \end{array} \right.$

If the Fourier series for  $f(x)$  converges in  $(-l, l)$

then  $\frac{1}{l} \int_{-l}^l \{f(x)\}^2 dx = \frac{a_0^2}{2} + \sum_{n=1}^{\infty} (a_n^2 + b_n^2)$ ; where

$a_0, a_n, b_n$  are Fourier constants.

Proof:-

we know

$$f(x) = \frac{a_0}{2} + \sum_{n=1}^{\infty} (a_n \cos \frac{n\pi x}{l} + b_n \sin \frac{n\pi x}{l})$$

where  $a_0 = \frac{1}{l} \int_{-l}^l f(x) dx$  ——— ①

$$a_n = \frac{1}{l} \int_{-l}^l f(x) \cos \frac{n\pi x}{l} dx$$

$$b_n = \frac{1}{l} \int_{-l}^l f(x) \sin \frac{n\pi x}{l} dx.$$

Now multiplying both sides of (i) by  $f(x)$ , then integrating from  $-l$  to  $l$ .

$$\int_{-l}^l \{f(x)\}^2 dx = \frac{a_0}{2} \int_{-l}^l f(x) dx + \sum_{n=1}^{\infty} \left( a_n \int_{-l}^l f(x) \cos \frac{n\pi x}{l} dx + b_n \int_{-l}^l f(x) \sin \frac{n\pi x}{l} dx \right).$$

$$= \frac{a_0}{2} \cdot a_0 l + \sum_{n=1}^{\infty} (a_n \cdot a_n l + b_n \cdot b_n l)$$

$$\text{or, } \frac{1}{l} \int_{-l}^l \{f(x)\}^2 dx = \frac{a_0^2}{2} + \sum_{n=1}^{\infty} (a_n^2 + b_n^2) \quad \text{proved.}$$



Prob:1: Expand in Fourier sine and cosine series of the function  $f(x) = x + x^2$  in the interval  $-\pi < x < \pi$ . Also show that

$$\frac{\pi^2}{6} = 1 + \frac{1}{2^2} + \frac{1}{3^2} + \frac{1}{4^2} + \frac{1}{5^2} + \dots$$

A:- We have  $f(x) = x + x^2$ ;  $-\pi < x < \pi$

In the interval  $-\pi < x < \pi$ , Fourier series is

$$f(x) = \frac{a_0}{2} + \sum_{n=1}^{\infty} (a_n \cos nx + b_n \sin nx) \quad \text{--- (1)}$$

where  $a_0 = \frac{1}{\pi} \int_{-\pi}^{\pi} f(x) dx$  ~~is given~~

$$= \frac{1}{\pi} \int_{-\pi}^{\pi} (x + x^2) dx = \frac{1}{\pi} \left[ \frac{x^2}{2} + \frac{x^3}{3} \right]_{-\pi}^{\pi}$$

$$= \frac{1}{\pi} \left[ \left( \frac{\pi^2}{2} + \frac{\pi^3}{3} \right) - \left( \frac{\pi^2}{2} - \frac{\pi^3}{3} \right) \right]$$

$$= \frac{1}{\pi} \cdot \frac{2\pi^3}{3} = \frac{2}{3} \pi^2.$$

$$a_n = \frac{1}{\pi} \int_{-\pi}^{\pi} f(x) \cos nx dx$$

$$= \frac{1}{\pi} \int_{-\pi}^{\pi} (x + x^2) \cos nx dx.$$

$$= \frac{1}{\pi} \left[ (x + x^2) \cdot \frac{\sin nx}{n} - \int_{-\pi}^{\pi} (1 + 2x) \cdot \frac{\sin nx}{n} dx \right]$$

$$= \frac{1}{\pi} \left[ (x + x^2) \frac{\sin nx}{n} + \frac{\cos nx}{n^2} - \int_{-\pi}^{\pi} 2x \frac{\sin nx}{n} dx \right]$$

$$= \frac{1}{\pi} \left[ (x+x^2) \frac{\sin nx}{n} + \frac{\cos nx}{n^2} - \left\{ 2x \cdot \frac{\cos nx}{n^2} - \int_{-\pi}^{\pi} 2 \cdot \left( -\frac{\cos nx}{n^2} \right) dx \right\} \right]$$

$$= \frac{1}{\pi} \left[ (x+x^2) \frac{\sin nx}{n} + \frac{\cos nx}{n^2} + 2x \cdot \frac{\cos nx}{n^2} + \frac{2 \sin nx}{n^3} \right]_{-\pi}^{\pi}$$

$$= \frac{1}{\pi} \left[ \left( 0 + \frac{\cos n\pi}{n^2} + 2\pi \frac{\cos n\pi}{n^2} + 0 \right) - \left( 0 + \frac{\cos n\pi}{n^2} - \frac{2\pi \cos n\pi}{n^2} \right) \right]$$

$$= \frac{1}{\pi} \left[ \frac{(-1)^n}{n^2} + 2\pi \cdot \frac{(-1)^n}{n^2} - \frac{(-1)^n}{n^2} + 2\pi \frac{(-1)^n}{n^2} \right]$$

$$= \frac{1}{\pi} \cdot 4\pi \frac{(-1)^n}{n^2} = \frac{4(-1)^n}{n^2}$$

Now

$$b_n = \frac{1}{\pi} \int_{-\pi}^{\pi} f(x) \sin nx \, dx$$

$$= \frac{1}{\pi} \int_{-\pi}^{\pi} (x+x^2) \sin nx \, dx$$

$$= \frac{1}{\pi} \left[ -(x+x^2) \frac{\cos nx}{n} + \int_{-\pi}^{\pi} (1+2x) \cdot \frac{\cos nx}{n} \, dx \right]$$

$$= \frac{1}{\pi} \left[ -(x+x^2) \frac{\cos nx}{n} + \frac{\sin nx}{n^2} + \left\{ 2x \cdot \frac{\sin nx}{n^2} - \int_{-\pi}^{\pi} 2 \cdot \frac{\sin nx}{n^2} \, dx \right\} \right]$$

$$= \frac{1}{\pi} \left[ -(x+x^2) \frac{\cos nx}{n} + \frac{\sin nx}{n^2} + 2x \frac{\sin nx}{n^2} + \frac{2 \cos nx}{n^3} \right]_{-\pi}^{\pi}$$

$$= \frac{1}{\pi} \left[ \left\{ -(\pi + \pi^2) \frac{\cos n\pi}{n} + 0 + 0 + \frac{2 \cos n\pi}{n^3} \right\} - \left\{ -(-\pi + \pi^2) \frac{\cos n\pi}{n} + 0 + 0 + \frac{2 \cos n\pi}{n^3} \right\} \right]$$

$$= \frac{1}{\pi} \left[ -(\pi + \pi^2) \frac{(-1)^n}{n} + \frac{2}{n^3} (-1)^n + (-\pi + \pi^2) \frac{(-1)^n}{n} - \frac{2}{n^3} (-1)^n \right]$$

$$= \frac{1}{\pi} \left[ \frac{(-1)^n}{n} (-\pi - \pi^2 - \pi + \pi^2) \right]$$

$$= \frac{1}{\pi} (-2\pi) \cdot \frac{(-1)^n}{n} = -2 \frac{(-1)^n}{n}$$

Now putting  $a_0, a_n, b_n$  in (i);

$$f(x) = \frac{1}{2} \cdot \frac{2}{3} \pi^2 + \sum_{n=1}^{\infty} \left[ \frac{4(-1)^n}{n^2} \cos nx - \frac{2(-1)^n}{n} \sin nx \right]$$

$$= \frac{\pi^2}{3} + 4 \left\{ -\frac{1}{1^2} \cos x + \frac{1}{2^2} \cos 2x - \frac{1}{3^2} \cos 3x + \dots \right\} - 2 \left\{ -\frac{\sin x}{1} + \frac{\sin 2x}{2} - \frac{\sin 3x}{3} + \dots \right\}$$

$$f(x) = \frac{\pi^2}{3} - 4 \left( \frac{\cos x}{1^2} - \frac{\cos 2x}{2^2} + \frac{\cos 3x}{3^2} - \dots \right) + 2 \left( \frac{\sin x}{1} - \frac{\sin 2x}{2} + \frac{\sin 3x}{3} - \dots \right) \quad (2)$$

2nd part: At the end points  $x = \pm \pi$ .

$$\begin{aligned} f(\pi) &= \frac{1}{2} [f(-\pi+0) + f(\pi-0)] \\ &= \frac{1}{2} [-\pi + \pi^2 + \pi + \pi^2] \\ &= \frac{2\pi^2}{2} = \pi^2. \end{aligned}$$

$f(x) = \frac{1}{2} [f(x) + f(x)]$   
 $\therefore f(\pm\pi) = \frac{1}{2} [f(-\pi+0) + f(\pi-0)]$   
 Since  $f(x) = x + x^2$

Now putting  $x = \pi$  in (2);

$$f(\pi) = \frac{\pi^2}{3} - 4 \left( -\frac{1}{1^2} - \frac{1}{2^2} - \frac{1}{3^2} - \dots \right) + 2(0)$$

$$\pi^2 - \frac{\pi^2}{3} = \frac{\pi^2}{3} + 4 \left( \frac{1}{1^2} + \frac{1}{2^2} + \frac{1}{3^2} + \dots \right)$$

$$\pi^2 - \frac{\pi^2}{3} = 4 \left( \frac{1}{1^2} + \frac{1}{2^2} + \frac{1}{3^2} + \dots \right)$$

$$2 \frac{\pi^2}{3} = 4 \left( \frac{1}{1^2} + \frac{1}{2^2} + \frac{1}{3^2} + \dots \right)$$

$$\frac{\pi^2}{6} = 1 + \frac{1}{2^2} + \frac{1}{3^2} + \frac{1}{4^2} + \frac{1}{5^2} + \dots \text{ proved}$$